verifying parallel map kernel for grid execution

pmap.v
@@ -1,13 +1,14 @@
 Require Import GPUCSL.
-
 Section Map.
 Local Notation TID := (Var 0).
-Local Notation ARR := (Var 1).
-Local Notation X := (Var 2).
-Local Notation Y := (Var 3).
-Local Notation I := (Var 4).
+Local Notation BID := (Var 1).
+Local Notation ARR := (Var 2).
+Local Notation X := (Var 3).
+Local Notation Y := (Var 4).
+Local Notation I := (Var 5).
 
 Variable ntrd : nat.
+Variable nblk : nat.
 Variable len : nat.
 Hypothesis len_neq_0 : len <> 0.
 
@@ -15,21 +16,26 @@ Variable f : nat -> Z.
 
 Local Close Scope exp_scope.
 
-Definition inv (i : nat) :=
-  Ex ix, !(I === Enum' (ix * ntrd + i)) ** !(Apure (ix * ntrd + i < len + ntrd)%nat) **
-     nth i (distribute ntrd (Gl ARR) (ix * ntrd) (fun i => f i + 1)%Z (nt_step ntrd) 0) emp **
-     nth i (distribute ntrd (Gl ARR) (len - (ix * ntrd)) (fun i => f i) (nt_step ntrd) (ix * ntrd)) emp.
+Local Notation nt_gr := (ntrd * nblk).
 
-Definition map_ker (i : nat) :=
-  I ::= TID%Z;;
-  WhileI  (inv i) (I < Z.of_nat len) (
+Definition inv (i : nat) (arr : Z) :=
+  Ex ix, 
+    !(ARR === arr) **
+    !(I === Enum' (ix * nt_gr + i)) **
+    !(Apure (ix * nt_gr + i < len + nt_gr)%nat) **
+    nth i (distribute nt_gr (Gl ARR) (ix * nt_gr) (fun i => f i + 1)%Z (nt_step nt_gr) 0) emp **
+    nth i (distribute nt_gr (Gl ARR) (len - (ix * nt_gr)) (fun i => f i) (nt_step nt_gr) (ix * nt_gr)) emp.
+
+Definition map_ker (i : nat) (arr : Z) :=
+  I ::= (TID +C BID *C Z.of_nat ntrd);;
+  WhileI  (inv i arr) (I < Z.of_nat len) (
     X ::= [Gl ARR +o I] ;;
     [Gl ARR +o I] ::= X + 1%Z ;;
-    I ::= I + Z.of_nat ntrd%Z
+    I ::= I +C Z.of_nat ntrd *C Z.of_nat nblk
   )%exp.
 
-Variable tid : Fin.t ntrd.
 Hypothesis ntrd_neq0 : ntrd <> 0.
+Hypothesis nblk_neq0 : nblk <> 0.
 
 Ltac unfold_pures :=
   repeat lazymatch goal with
@@ -47,15 +53,44 @@ Ltac sep_rewrite_r lem :=
   end; erewrite <-lem; cbv beta. 
 
 Hint Rewrite Nat2Z.inj_add Nat2Z.inj_mul Nat2Z.inj_succ div_Zdiv : sep.
-Lemma map_correct :
-  CSL (fun n => default ntrd) tid
-  (List.nth (nat_of_fin tid) (distribute ntrd (Gl ARR) len f (nt_step ntrd) 0) emp **
-   !(TID === Z_of_fin tid))
-  (map_ker (nat_of_fin tid))
-  (List.nth (nat_of_fin tid) (distribute ntrd (Gl ARR) len (fun x => f x + 1)%Z (nt_step ntrd) 0) emp).
+
+Require Import LibTactics.
+
+Notation zf i := (Z_of_fin i).
+
+Lemma nt_gr_neq_0 : nt_gr <> 0.
 Proof.
-  assert (Htid : nat_of_fin tid < ntrd) by (destruct (Fin.to_nat _); simpl in *; auto).
-  unfold map_ker.
+  apply Nat.neq_mul_0; tauto.
+Qed.
+
+Require Import Psatz.
+
+Lemma id_lt_nt_gr i j n m : i < n -> j < m -> i + j * n < n * m.
+Proof.
+  intros.
+  assert (i + j * n < n + j * n) by omega.
+  assert (n + j * n <= n * m) by nia.
+  omega.
+Qed.
+
+Lemma nf_lt : forall n (i : Fin.t n), nf i < n.
+Proof.
+  introv; destruct Fin.to_nat; simpl; omega.
+Qed.
+
+Hint Resolve nt_gr_neq_0 id_lt_nt_gr nf_lt.
+
+
+Lemma map_correct : forall (tid : Fin.t ntrd) (bid : Fin.t nblk) (arr : Z), 
+  CSL (fun n => default ntrd) tid
+  (!(ARR === arr) ** 
+   List.nth (nf tid + nf bid * ntrd) (distribute nt_gr (Gl arr) len f (nt_step nt_gr) 0) emp **
+   !(BID === zf bid) ** !(TID === zf tid))
+  (map_ker (nf tid + nf bid * ntrd) arr)
+  (List.nth (nf tid + nf bid * ntrd) (distribute nt_gr (Gl arr) len (fun x => f x + 1)%Z (nt_step nt_gr) 0) emp).
+Proof.
+  (* assert (Htid : nat_of_fin tid < ntrd) by (destruct (Fin.to_nat _); simpl in *; auto). *)
+  unfold map_ker; introv.
   eapply rule_seq.
   { hoare_forward; intros ? ? H'.
     destruct H' as [v H'].
@@ -64,77 +99,109 @@ Proof.
   { unfold inv; eapply Hbackward.
     Focus 2.
     { intros s h H; apply ex_lift_l_in in H as [x H]; sep_split_in H.
-      change_in H; [unfold_pures|]. 
-
-      sep_rewrite_in skip_arr_unfold' H; [|try omega..]. 
-      2: rewrite HP0 in l; apply Nat2Z.inj_lt in l; omega.
-      apply H. sep_combine_in H. ex_intro x H. simpl in H. exact H. } Unfocus.
+      change_in H.
+      { unfold_pures.
+        sep_rewrite_in skip_arr_unfold' H; [|try first [omega | eauto]..]. 
+      2: zify; omega.
+      apply H. } 
+      sep_combine_in H. ex_intro x H. simpl in H. exact H. } Unfocus.
     
     hoare_forward.
     eapply rule_seq. 
     { autorewrite with sep. eapply Hbackward. 
       Focus 2.
-      intros s h H.
-      sep_split_in H.
-      change_in H.
-      assert ((Gl ARR +o (Z.of_nat x * Z.of_nat ntrd + Z_of_fin tid)%Z ===l Gl ARR +o I)%exp s (emp_ph loc)).
-      unfold_pures; unfold_conn; simpl; f_equal; omega.
-      sep_rewrite_in (mps_eq1) H; [|exact H0]. exact H.
-      sep_combine_in H; exact H.
+      { intros s h H.
+        sep_split_in H.
+        change_in H.
+        { assert ((Gl ARR +o (Zn x * (Zn ntrd * Zn nblk) + (zf tid + zf bid * Zn ntrd))%Z ===l
+                  Gl ARR +o I)%exp s (emp_ph loc)).
+          { unfold_pures; unfold_conn; simpl; f_equal; omega. }
+          sep_rewrite_in (mps_eq1) H; [|exact H0]. exact H. }
+          sep_combine_in H; exact H. } Unfocus.
       hoare_forward; try (apply inde_distribute; auto; repeat (constructor; prove_indeE)).
       intros ? ? H; apply H. }
-
+    
     eapply rule_seq.
     { hoare_forward.
       intros ? ? H; apply H. }
     
     eapply Hforward.
     { hoare_forward.
-      intros ? ? H; destruct H as [v H]. subA_normalize_in H. simpl in H. ex_intro v H. exact H. }
+      intros ? ? H; destruct H as [v H].
+      subA_normalize_in H. simpl in H. ex_intro v H. exact H. }
     
     unfold inv; intros s h H. destruct H as (v & H); simpl in H.
-    sep_split_in H; unfold_pures; subst.
+    sep_split_in H. unfold_pures; subst.
     exists (S x); autorewrite with sep.
-    sep_split.
-    - unfold_conn; simpl. rewrite Z.mul_succ_l. omega.
-    - unfold_conn. apply Nat2Z.inj_lt; autorewrite with sep; rewrite Z.mul_succ_l; omega.
-    - sep_rewrite_r skip_arr_fold'; try omega.
-      sep_normal. simpl. repeat sep_cancel.
-      rewrite (plus_comm ntrd (x * ntrd)), Nat.sub_add_distr, (plus_comm _ ntrd).
-      apply scC. sep_cancel.
-      autorewrite with sep. sep_cancel. }
+    sep_split; try now (unfold_conn; simpl; auto; nia).
+    sep_rewrite_r skip_arr_fold'; try omega; eauto.
+    sep_normal; simpl; repeat sep_cancel.
+    autorewrite with sep. repeat sep_cancel.
+    cuts_rewrite (len - (nt_gr + x * nt_gr) = len - x * nt_gr - nt_gr); auto.
+    zify; omega. }
 
-  { unfold inv; intros s h H. apply ex_lift_l_in in H as [x H]. sep_split_in H.
-    unfold_pures.
-    rewrite HP0 in n; rewrite <-Nat2Z.inj_lt in n.
-    assert (x * ntrd <= len \/ len < x * ntrd) as [|] by omega.
-    - apply scC in H; sep_rewrite_in nth_dist_nil H; try omega; eauto.
-      2: instantiate (1 :=len - x * ntrd); intros j Hj; unfold nt_step;
+  { unfold inv; intros s h H. apply ex_lift_l_in in H as [x H]. sep_split_in H. unfold_pures.
+    rewrite HP1 in n; rewrite <-Nat2Z.inj_lt in n.
+    assert (len - x * nt_gr <= nf tid + nf bid * ntrd) by (zify; omega).
+    assert (nf tid + nf bid * ntrd < nt_gr) by auto.
+    apply scC in H; sep_rewrite_in nth_dist_nil H; try omega; eauto.
+    2: instantiate (1 :=len - x * nt_gr); intros j Hj; unfold nt_step.
+    2: rewrite plus_comm, Nat.mod_add; auto; rewrite Nat.mod_small; auto; try (zify; omega).
+    rewrite minus_diag in H; simpl in H.
+    rewrite nth_nseq in H.
+    Lemma distribute_eq e e' stk i nt n f' dist:
+      i < nt -> (forall i, dist i < nt) ->
+      (e ===l e') stk (emp_ph loc) ->
+      forall s, stk ||= nth i (distribute nt e n f' dist s) emp <=>
+                        nth i (distribute nt e' n f' dist s) emp.
+    Proof.
+      induction n; simpl; intros; [split; eauto|].
+      rewrite !nth_add_nth; [|rewrite distribute_length; eauto..].
+      destruct beq_nat; eauto.
+      assert ((e +o Zn s ===l e' +o Zn s) stk (emp_ph loc)).
+      { unfold_conn_all; simpl in *; rewrite H1; eauto. }
+      rewrite mps_eq1; [|exact H2].
+      split; intros; sep_cancel; apply IHn; auto.
+    Qed.
+    assert ((Gl arr ===l Gl ARR) s (emp_ph loc)) by (unfold_conn; simpl; congruence).
+    sep_rewrite distribute_eq; eauto.
+    assert (x * nt_gr <= len \/ len < x * nt_gr) as [|] by omega.
+    - apply scC in H; sep_rewrite_in nth_dist_ext H; try omega; auto.
+      2: instantiate (1 :=len - x * nt_gr); intros j Hj; simpl; unfold nt_step;
          rewrite plus_comm, Nat.mod_add; auto; rewrite Nat.mod_small; auto; try omega.
-      rewrite minus_diag in H; simpl in H.
-      apply scC in H; sep_rewrite_in nth_dist_ext H; try omega; eauto.
-      2: instantiate (1 :=len - x * ntrd); intros j Hj; simpl; unfold nt_step;
-         rewrite plus_comm, Nat.mod_add; auto; rewrite Nat.mod_small; auto; try omega.
-      cutrewrite (x * ntrd + (len - x * ntrd) = len) in H; [|omega].
-      rewrite nth_nseq in H; destruct leb; sep_normal_in H; auto.
-    - cutrewrite (len - x * ntrd = 0) in H; [|omega].
-      cutrewrite (x * ntrd = len + (x * ntrd - len)) in H; [|omega].
+      cutrewrite (x * nt_gr + (len - x * nt_gr) = len) in H; [|omega].
+
+      destruct leb; sep_normal_in H; sep_cancel.
+    - (* apply scC in H; sep_rewrite nth_dist_ext; try omega; auto. *)
+      (* cutrewrite (len - x * ntrd = 0) in H; [|omega]. *)
+      cutrewrite (x * nt_gr = len + (x * nt_gr - len)) in H; [|omega].
       sep_rewrite_in_r nth_dist_ext H; try omega; eauto.
-      simpl in H; rewrite nth_nseq in H; destruct leb; sep_normal_in H; sep_cancel.
+      destruct leb; sep_normal_in H; sep_cancel.
       unfold nt_step; simpl; intros j Hj Hc.
-      assert (len + j + ntrd < (S x) * ntrd) by (simpl; omega).
-      assert (x * ntrd + j + (nf tid) < len + j + ntrd ) by omega.
-      let t := (eval simpl in (Nat.mod_add (len + j) 1 ntrd)) in pose proof t. rewrite mult_1_l in H3.
-      rewrite (Nat.div_mod (len + j + ntrd) ntrd ntrd_neq0), H3 in H1, H2; auto.
-      assert (x * ntrd  < ntrd * ((len + j + ntrd) / ntrd)) by omega.
-      assert (ntrd * ((len + j + ntrd) / ntrd) < S x * ntrd) by omega.
-      rewrite mult_comm in H4; apply Nat.mul_lt_mono_pos_l in H4; try omega.
-      rewrite mult_comm in H5; apply Nat.mul_lt_mono_pos_r in H5; omega. }
+      assert (len + j + nt_gr < (S x) * nt_gr) by (simpl; omega).
+      assert (x * nt_gr + j + (nf tid + nf bid * ntrd) < len + j + nt_gr) by omega.
+      let t := (eval simpl in (Nat.mod_add (len + j) 1 nt_gr)) in pose proof t.
+      rewrite mult_1_l in H6.
+      rewrite (Nat.div_mod (len + j + nt_gr) nt_gr), H6 in H4, H5; auto.
+      assert (x * nt_gr  < nt_gr * ((len + j + nt_gr) / nt_gr)) by omega.
+      assert (nt_gr * ((len + j + nt_gr) / nt_gr) < S x * nt_gr) by omega.
+      rewrite mult_comm in H7; apply Nat.mul_lt_mono_pos_l in H7; try omega.
+      rewrite mult_comm in H8; apply Nat.mul_lt_mono_pos_r in H8; omega. }
 
   {  intros s h H; unfold inv; exists 0; simpl.
      sep_split_in H; unfold_pures; sep_split.
-     - unfold_conn; simpl; congruence.
-     - unfold_conn; omega.
-     - rewrite <-minus_n_O, nth_nseq; destruct leb; sep_normal; sep_cancel. }
+     - unfold_conn; simpl; eauto.
+     - unfold_conn; simpl; autorewrite with sep; congruence.
+     - unfold_conn. assert (nf tid + nf bid * ntrd < nt_gr) by auto. omega.
+     - assert ((Gl ARR ===l Gl arr) s (emp_ph loc)) by (unfold_conn; simpl; congruence).
+       sep_rewrite distribute_eq; eauto.
+       rewrite <-minus_n_O, nth_nseq; destruct leb; sep_normal; sep_cancel. }
 Qed.
+
+Definition map' : cmd.
+  pose (map_ker 0) as map'; unfold map_ker, WhileI in map'; exact map'.
+Defined.
+
+Definition block_pre := distribute nblk 
+
 End Map.
